<?xml version="1.0" encoding = "UTF-8"?>
<rdf:RDF xmlns:rdf="http://www.w3.org/1999/02/22-rdf-syntax-ns#"
    xmlns:rdfs="http://www.w3.org/2000/01/rdf-schema#" xmlns:owl="http://www.w3.org/2002/07/owl#"
    xmlns:skos="http://www.w3.org/2004/02/skos/core#" xmlns:dc="http://purl.org/dc/elements/1.1/"
    xmlns:dct="http://purl.org/dc/terms/"
    xmlns:foaf="http://xmlns.com/foaf/0.1/"
    xmlns:cc="http://creativecommons.org/ns#"
    xmlns:vann="http://purl.org/vocab/vann/">

    <owl:Ontology rdf:about="https://d-nb.info/standards/vocab/gnd/type-of-coordinates#">
		<owl:imports rdf:resource="http://www.w3.org/2004/02/skos/core#" />
        <rdf:type rdf:resource="http://www.w3.org/2004/02/skos/core#ConceptScheme"/>
        <dc:title xml:lang="en">GND Type of Coordinates</dc:title>
        <dc:title xml:lang="de">GND-Koordinatentyp</dc:title>
		<dc:description xml:lang="en">GND Type of Coordinates is a skos:ConceptScheme listing possible values for
		types of coordinates in date in the Integrated Authority File (Gemeinsame Normdatei, GND).
		The four concepts mirror the way geographic coordinates are specified in the GND database: The
		coordinates can be saved either in analogue or decimal format and further it can be specified
		if the coordinates are precise (e. g. if the exact position of an object is known) or imprecise
		(e. g. when the source does not supply precis information).</dc:description>
		<dc:description xml:lang="de">GND-Koordinatentyp ist ein skos:ConceptScheme das die möglichen Werte
		für Koordinatentypen in den Daten der Gemeinsamen Normdatei (GND) aufführt. Die vier Begriffe entsprechen
		die Art, wie geografische Koordinaten gespeichert werden in der GND: Sie können entweder in analoger
		oder dezimaler Darstellung gespeichert werden und weiter kann spezifiziert werden, ob sie exakt (z. B.
		wenn die genaue Position eines Objekts bekannt sind) oder ungenau (z. B. wenn die Quelle keine genaue
		Information liefert) sind.</dc:description>
        <!-- For Linked Open Vocabularies -->
        <vann:preferredNamespaceUri>https://d-nb.info/standards/vocab/gnd/type-of-coordinates#</vann:preferredNamespaceUri>
        <vann:preferredNamespacePrefix>gnd-tc</vann:preferredNamespacePrefix>
        
        <!-- Versioning information -->
		<dct:created rdf:datatype="http://www.w3.org/2001/XMLSchema#date">2012-06-30</dct:created>
        <dct:issued rdf:datatype="http://www.w3.org/2001/XMLSchema#date">2022-09-27</dct:issued>
        <dct:modified rdf:datatype="http://www.w3.org/2001/XMLSchema#dateTime">2022-04-06T10:29:00+02:00</dct:modified>
        <dct:available rdf:datatype="http://www.w3.org/2001/XMLSchema#date">2022-09-27</dct:available>
        <owl:versionInfo>1.3</owl:versionInfo>
		<rdfs:comment xml:lang="en">
            Changes from 2019-10-15 to 2022-09-27
            Fix vann:preferredNamespacePrefix from gnd-sc to gnd-tc
			Changes from 2017-09-12 to 2019-10-15
			All d-nb.info-URIs changed from http to https
		</rdfs:comment>
        <owl:versionIRI rdf:resource="https://d-nb.info/standards/vocab/gnd/type-of-coordinates_20191015" />
		<owl:priorVersion rdf:resource="http://d-nb.info/standards/vocab/gnd/type-of-coordinates_20170912" />

        <!-- Rights information -->
        <dct:rights>Copyright 2012-2022 Deutsche Nationalbibliothek</dct:rights>
        <cc:license rdf:resource="http://creativecommons.org/publicdomain/zero/1.0/" />
        <dct:license rdf:resource="http://creativecommons.org/publicdomain/zero/1.0/"/>
		<dct:creator rdf:resource="#alexanderHaffner" />
        <dct:publisher rdf:resource="http://ld.zdb-services.de/resource/organisations/DE-101" />
    </owl:Ontology>

    <!-- Stubs for creator -->
	<foaf:Person rdf:about="#alexanderHaffner">
		<rdfs:label>Alexander Haffner</rdfs:label>
		<owl:sameAs rdf:resource="https://d-nb.info/gnd/1037982762"/>
	</foaf:Person>
    
    <owl:Class rdf:about="https://d-nb.info/standards/vocab/gnd/type-of-coordinates#TypeOfCoordinatesValue">
        <rdfs:subClassOf rdf:resource="http://www.w3.org/2004/02/skos/core#Concept"/>
        <owl:equivalentClass>
            <owl:Restriction>
                <owl:onProperty rdf:resource="http://www.w3.org/2004/02/skos/core#inScheme"/>
                <owl:hasValue rdf:resource="https://d-nb.info/standards/vocab/gnd/type-of-coordinates#"/>
            </owl:Restriction>
        </owl:equivalentClass>
        <rdfs:label xml:lang="en">GND Type of Coordinates Value</rdfs:label>
        <rdfs:label xml:lang="de">Werte für GND-Koordinatentyp</rdfs:label>
        <rdfs:comment xml:lang="en">The possible members of this class is restricted to those skos:Concepts
            that are in the Concept Scheme &lt;https://d-nb.info/standards/vocab/gnd/type-of-coordinates#&gt;.</rdfs:comment>
        <rdfs:comment xml:lang="de">Die möglichen Instanzen dieser Klasse sind beschränkt auf diejenigen
            skos:Concepts, die zum Concept Scheme &lt;https://d-nb.info/standards/vocab/gnd/type-of-coordinates#&gt; gehören.</rdfs:comment>    </owl:Class>
    
    <skos:Concept rdf:about="https://d-nb.info/standards/vocab/gnd/type-of-coordinates#analogRepresentationOfImpreciseCoordinates">
        <skos:inScheme rdf:resource="https://d-nb.info/standards/vocab/gnd/type-of-coordinates#"/>
        <skos:prefLabel xml:lang="de">Analoge Darstellung ungenauer Koordinaten</skos:prefLabel>
        <skos:prefLabel xml:lang="en">Analog representation of imprecise coordinates</skos:prefLabel>
    </skos:Concept>
    <skos:Concept rdf:about="https://d-nb.info/standards/vocab/gnd/type-of-coordinates#analogRepresentationOfPreciseCoordinates">
        <skos:inScheme rdf:resource="https://d-nb.info/standards/vocab/gnd/type-of-coordinates#"/>
        <skos:prefLabel xml:lang="de">Analoge Darstellung genauer Koordinaten</skos:prefLabel>
        <skos:prefLabel xml:lang="en">Analog representation of precise coordinates</skos:prefLabel>
    </skos:Concept>
    <skos:Concept rdf:about="https://d-nb.info/standards/vocab/gnd/type-of-coordinates#decimalRepresentationOfImpreciseCoordinates">
        <skos:inScheme rdf:resource="https://d-nb.info/standards/vocab/gnd/type-of-coordinates#"/>
        <skos:prefLabel xml:lang="de">Dezimale Darstellung ungenauer Koordinaten</skos:prefLabel>
        <skos:prefLabel xml:lang="en">Decimal representation of imprecise coordinates</skos:prefLabel>
    </skos:Concept>
    <skos:Concept rdf:about="https://d-nb.info/standards/vocab/gnd/type-of-coordinates#decimalRepresentationOfPreciseCoordinates">
        <skos:inScheme rdf:resource="https://d-nb.info/standards/vocab/gnd/type-of-coordinates#"/>
        <skos:prefLabel xml:lang="de">Dezimale Darstellung genauer Koordinaten</skos:prefLabel>
        <skos:prefLabel xml:lang="en">Decimal representation of precise coordinates</skos:prefLabel>
    </skos:Concept>	
</rdf:RDF>
